added refine_BagADT_QSInsert

examples/DnsServer/Dns.v
@@ -2,33 +2,33 @@ Require Import AutoDB BagADT.
 Require Import Vector Ascii Bool Bvector List.
 
 Record label :=
-  { length : N;
+  { length : nat;
     word : string }.
 Definition name := list label.
 
-(* Name or pointer offset to a name *)
-Inductive pname :=  fullname : name -> pname | pointername : N -> pname.
+Inductive type := A | CNAME | NS | MX.
+Inductive class := IN | CH | HS.
 
 Record question :=
   { qname : name;
-    qtype : N;
-    qclass : N }.
+    qtype : type;
+    qclass : class }.
 
 Record answer :=
-  { aname : name; (* `pname` if we allow compression *)
-    atype : N;
-    aclass : N;
-    ttl : N;
-    rdlength : N;
-    rdata : list ascii }.
+  { aname : name;
+    atype : type;
+    aclass : class;
+    ttl : nat;
+    rdlength : nat;
+    rdata : string }.
 
 Record packet :=
-  { id : N;
-    flags : Bvector 16; (* 16 bits of boolean *)
-    qdcount : N;
-    ancount : N;
-    nscount : N;
-    arcount : N;
+  { id : Bvector 16;
+    flags : Bvector 16;
+    qdcount : nat;
+    ancount : nat;
+    nscount : nat;
+    arcount : nat;
     questions : question; (* `list question` in case we can have multiple questions? *)
     answers : list answer;
     authority : list answer;
@@ -46,67 +46,179 @@ Definition DnsSchema :=
   Query Structure Schema
         [ relation sCOLLECTIONS has
                    schema <sNAME :: name,
-                           sTTL :: N,
-                           sCLASS :: N,
-                           sTYPE :: N,
-                           sDLENGTH :: N,
-                           sDATA :: string> ]
+                           sTYPE :: type,
+                           sCLASS :: class,
+                           sTTL :: nat,
+                           sDATA :: string>
+          where (fun t t' =>
+                   t!sNAME = t'!sNAME -> t!sTYPE <> CNAME /\ t'!sTYPE <> CNAME)]
         enforcing [ ].
-(*
-     + one CNAME record exists, optionally accompanied by SIG, NXT, and
-       KEY RRs,
-     + one or more records exist, none being CNAME records,
-     + the name exists, but has no associated RRs of any type,
-     + the name does not exist at all.
-*)
 
 Definition DnsTuple := TupleDef DnsSchema sCOLLECTIONS.
 Definition DnsSig : ADTSig :=
   ADTsignature {
       Constructor "Init" : unit -> rep,
+      Method "AddData" : rep x DnsTuple -> rep x bool,
       Method "Process" : rep x packet -> rep x packet
   }.
 
-Definition prefix (p s : name) := exists ps, List.app p ps = s.
+Definition beq_string (p s : string) := if string_dec p s then true else false.
+Definition beq_label (p s : label) :=
+  andb (beq_nat (length p) (length s)) (beq_string (word p) (word s)).
+
+Definition prefixProp (p s : name) := exists ps, List.app p ps = s.
+Fixpoint prefixBool (p s : name) :=
+  match p, s with
+    | List.nil, _ => true 
+    | List.cons p' ps', List.cons s' ss' => andb (beq_label p' s') (prefixBool ps' ss')
+    | _, _ => false
+  end.
 
 Definition upperbound (r : DnsTuple) (rs : list DnsTuple) :=
   forall r', List.In r' rs -> List.length r!sNAME >= List.length r'!sNAME.
- 
-Definition cname : N := 5 % N.
 
 Lemma zero_lt_sixteen : lt 0 16. omega. Qed.
-Definition buildempty (input : packet) : packet :=
-  {| id := id input;
-     flags := replace_order (flags input) zero_lt_sixteen true; (* set QR bit *)
-     qdcount := qdcount input;
+Definition buildempty (p : packet) :=
+  {| id := id p;
+     flags := replace_order (flags p) zero_lt_sixteen true; (* set QR bit *)
+     qdcount := qdcount p;
      ancount := 0;
      nscount := 0;
      arcount := 0;
-     questions := questions input; (*list question*)
+     questions := questions p;
      answers := List.nil;
      authority := List.nil;
      additional := List.nil |}.
 
-Variable addns : packet -> DnsTuple -> packet.
-Variable addrr : packet -> DnsTuple -> packet.
-Variable rec : packet.
-Variable EnsembleEq : forall A, Ensemble A -> list A -> Prop.
+Definition toAnswer (t: DnsTuple) :=
+  {| aname := t!sNAME;
+     atype := t!sTYPE;
+     aclass := t!sCLASS;
+     ttl := t!sTTL;
+     rdlength := 0 (* INCORRECT *);
+     rdata := t!sDATA |}.
+
+Definition addan (p : packet) (t : DnsTuple) :=
+  {| id := id p;
+     flags := flags p;
+     qdcount := qdcount p;
+     ancount := (ancount p) + 1;
+     nscount := nscount p;
+     arcount := arcount p;
+     questions := questions p;
+     answers := (toAnswer t) :: answers p;
+     authority := authority p;
+     additional := additional p |}.
+
+Definition addns (p : packet) (t : DnsTuple) :=
+  {| id := id p;
+     flags := flags p;
+     qdcount := qdcount p;
+     ancount := ancount p;
+     nscount := (nscount p) + 1;
+     arcount := arcount p;
+     questions := questions p;
+     answers := answers p;
+     authority := (toAnswer t) :: (authority p);
+     additional := additional p |}.
+
+Fixpoint Fix A R (i : nat) (body : (A -> R) -> A -> R) (base : R) (arg : A) :=
+  match i with
+    | O => base
+    | S i' => body (Fix i' body base) arg
+  end.
+
+Add Parametric Morphism A R i
+: (@Fix A (Comp R) i)
+    with signature
+    (fun f g => forall a a' r, (forall b, refine (a b) (a' b)) -> refine (f a r) (g a' r))
+      ==> (@refine R) 
+      ==> (@eq A)
+      ==> (@refine R)
+      as refineFix.
+Proof.
+  simpl; induction i; intros; simpl.
+  - assumption.
+  - apply H.
+    apply IHi.
+    + apply H.
+    + apply H0.
+Qed.
+
+Arguments Fix : simpl never.
+
+Notation "'Filter' xs | p" := (Pick (fun xs' => forall x, List.In x xs' <-> List.In x xs /\ p x)) (at level 70) : comp_scope.
+Notation "'if' p ->> s 'otherwise' ->> s' 'fi'" := (Bind (Pick (fun x => x = true <-> p)) (fun x => if x then s else s')) (at level 70).
+Notation "'unique' b , p ->> s 'otherwise' ->> s'" := 
+  (Bind (Pick (fun b' => forall b, b' = Some b <-> p)) (fun b' =>
+   match b' with
+     | Some b => s
+     | None => s'
+   end)) (at level 70).
 
 Definition DnsSpec : ADT DnsSig :=
   QueryADTRep DnsSchema {
     Def Constructor "Init" (_ : unit) : rep := empty,
+    update "AddData" (t : DnsTuple) : bool :=
+      Insert t into sCOLLECTIONS,
     query "Process" (p : packet) : packet :=
-      rs <- For (r in sCOLLECTIONS)
-         Where (prefix r!sNAME (qname (questions p)))
-         Return r;
-      bfrs <- { bfrs | forall r, List.In r bfrs <-> List.In r rs /\ upperbound r rs };
-      matched <- { matched | matched = true <-> forall b, List.In b bfrs -> (qname (questions p)) = b!sNAME }; 
-      if matched
-      then 
-        is_cname <- { is_cname | is_cname = true <-> exists b, List.In b bfrs -> b!sTYPE = cname };
-        if andb is_cname (negb (N.eqb (qtype (questions p)) cname))
-        then ret (List.fold_left addrr bfrs rec)
-        else ret (List.fold_left addrr bfrs (buildempty p))
-      else 
-        ret (List.fold_left addns bfrs (buildempty p))
+      let t := qtype (questions p) in
+      Fix 7 (fun (rec : name -> Comp packet) (n : name)  =>
+         rs <- For (r in sCOLLECTIONS)
+            Where (prefixProp r!sNAME n)
+            Return r;
+         bfrs <- Filter rs | (fun x : DnsTuple => upperbound x rs);
+         if forall b, List.In b bfrs -> n = b!sNAME ->> 
+           unique b, List.In b bfrs /\ b!sTYPE = CNAME /\ t <> CNAME ->>
+             bfrs' <- Filter bfrs | (fun x : DnsTuple => x!sTYPE = t);
+             p' <- rec b!sNAME;
+             ret (List.fold_left addan bfrs' p')
+           otherwise ->>
+             ret (List.fold_left addan bfrs (buildempty p))
+         otherwise ->> 
+           bfrs' <- Filter bfrs | (fun x : DnsTuple => x!sTYPE = NS);
+           ret (List.fold_left addns bfrs' (buildempty p))
+         fi
+      ) (ret (buildempty p)) (qname (questions p))
   }.
+
+Definition SearchTerm (s : name) (t : DnsSchema # sCOLLECTIONS) :=
+  prefixBool (t!sNAME) s.
+Definition DnsTerm :=
+  {| BagSearchTermType := name;
+     BagMatchSearchTerm := SearchTerm;
+     BagUpdateTermType := name;
+     BagApplyUpdateTerm := fun _ x => x |}.
+
+Lemma foo :
+  forall or (n : DnsTuple),
+  refine {b : bool | (forall tup' : @IndexedTuple (QSGetNRelSchemaHeading DnsSchema {| bindex := sCOLLECTIONS |}), (or!sCOLLECTIONS)%QueryImpl tup' -> n!sNAME = (indexedElement tup')!sNAME -> n!sTYPE <> CNAME /\ (indexedElement tup')!sTYPE <> CNAME)}
+         (ret true).
+
+Theorem DnsManual :
+  Sharpened DnsSpec.
+Proof.
+  unfold DnsSpec.
+  start honing QueryStructure.
+
+  hone representation using (@DelegateToBag_AbsR DnsSchema (icons DnsTerm (inil _))).
+  
+  hone constructor "Init".
+  {
+    simplify with monad laws.
+    rewrite refine_QSEmptySpec_Initialize_IndexedQueryStructure.
+    finish honing.
+  }
+  
+  hone method "AddData".
+  {
+    simplify with monad laws.
+  
+  hone method "Process".
+  {
+    simplify with monad laws.
+    implement_In.
+  }
+
+Defined.
+  FullySharpenQueryStructure DnsSchema Index.
